Tests.lean
@@ -8,6 +8,7 @@ import Tests.Direction
 import Tests.Examples
 import Tests.Grid
 import Tests.Invariance
+import Tests.Output
 import Tests.Parser
 import Tests.Random
 import Tests.Run
